powerpc/CombineOp.v
@@ -70,20 +70,9 @@ Function combine_cond (cond: condition) (args: list valnum) : option(condition *
   | _, _ => None
   end.
 
-Definition combine_comparison (c: comparison) (x y: valnum) : option bool :=
-  match c with
-  | Ceq => if eq_valnum x y then Some true else None
-  | Cle => if eq_valnum x y then Some true else None
-  | Cge => if eq_valnum x y then Some true else None
-  | Cne => if eq_valnum x y then Some false else None
-  | Clt => if eq_valnum x y then Some false else None
-  | Cgt => if eq_valnum x y then Some false else None
-  end.
-
 Definition combine_cond' (cond: condition) (args: list valnum) : option bool :=
   match cond, args with
-  | Ccomp c, x :: y :: nil => combine_comparison c x y
-  | Ccompu c, x :: y :: nil => combine_comparison c x y
+  | (Ccomp c | Ccompu c), x :: y :: nil => combine_comparison c x y
   | _, _ => None
   end.
 
