powerpc/CombineOpproof.v
@@ -125,50 +125,6 @@ Proof.
   simpl; eapply combine_compimm_eq_1_sound; eauto.
 Qed.
 
-Lemma combine_comparison_ccomp_sound:
-  forall c x y res res',
-  combine_comparison c x y = Some res' ->
-  eval_condition (Ccomp c) (valu x :: valu y :: nil) m = Some res ->
-  res = res'.
-Proof.
-  unfold combine_comparison. intros.
-  destruct c, (eq_valnum x y); inv H; destruct (valu y); inv H0;
-  try rewrite Int.eq_true; auto;
-  unfold Int.lt; rewrite zlt_false; auto; lia.
-Qed.
-
-Lemma combine_comparison_ccompu_sound:
-  forall c x y res res',
-  combine_comparison c x y = Some res' ->
-  eval_condition (Ccompu c) (valu x :: valu y :: nil) m = Some res ->
-  res = res'.
-Proof.
-  unfold combine_comparison. intros.
-  destruct c, (eq_valnum x y); inv H; destruct (valu y); inv H0;
-  try rewrite Int.eq_true; auto;
-  unfold Int.ltu; try rewrite zlt_false; auto; try lia;
-  destruct Archi.ptr64, (eq_block b b); inv H1.
-  destruct (Mem.valid_pointer m b (Ptrofs.unsigned i) || Mem.valid_pointer m b (Ptrofs.unsigned i - 1)); inv H0.
-  apply Ptrofs.eq_true.
-  destruct (Mem.valid_pointer m b (Ptrofs.unsigned i) && Mem.valid_pointer m b (Ptrofs.unsigned i)); inv H0. congruence.
-  destruct (Mem.valid_pointer m b (Ptrofs.unsigned i) || Mem.valid_pointer m b (Ptrofs.unsigned i - 1)); inv H0.
-  rewrite Ptrofs.eq_true; auto.
-  destruct (Mem.valid_pointer m b (Ptrofs.unsigned i) && Mem.valid_pointer m b (Ptrofs.unsigned i)); inv H0; congruence.
-  destruct (Mem.valid_pointer m b (Ptrofs.unsigned i) || Mem.valid_pointer m b (Ptrofs.unsigned i - 1)); inv H0.
-  unfold Ptrofs.ltu. rewrite zlt_false; auto. lia.
-  destruct (Mem.valid_pointer m b (Ptrofs.unsigned i) && Mem.valid_pointer m b (Ptrofs.unsigned i)); inv H0.
-  destruct (Mem.valid_pointer m b (Ptrofs.unsigned i) || Mem.valid_pointer m b (Ptrofs.unsigned i - 1)); inv H0.
-  unfold Ptrofs.ltu. rewrite zlt_false; auto. lia.
-  destruct (Mem.valid_pointer m b (Ptrofs.unsigned i) && Mem.valid_pointer m b (Ptrofs.unsigned i)); inv H0.
-  destruct (Mem.valid_pointer m b (Ptrofs.unsigned i) || Mem.valid_pointer m b (Ptrofs.unsigned i - 1)); inv H0.
-  unfold Ptrofs.ltu. rewrite zlt_false; auto. lia.
-  destruct (Mem.valid_pointer m b (Ptrofs.unsigned i) && Mem.valid_pointer m b (Ptrofs.unsigned i)); inv H0.
-  destruct (Mem.valid_pointer m b (Ptrofs.unsigned i) || Mem.valid_pointer m b (Ptrofs.unsigned i - 1)); inv H0.
-  unfold Ptrofs.ltu. rewrite zlt_false; auto. lia.
-  destruct (Mem.valid_pointer m b (Ptrofs.unsigned i) && Mem.valid_pointer m b (Ptrofs.unsigned i)); inv H0.
-Qed.
-
-
 Theorem combine_cond'_sound:
   forall cond args res res',
   combine_cond' cond args = Some res' ->
@@ -177,8 +133,8 @@ Theorem combine_cond'_sound:
 Proof.
   intros.  unfold combine_cond' in *.
   destruct cond; inv H; destruct args; inv H2; destruct args; inv H1; destruct args; inv H2.
-  apply (combine_comparison_ccomp_sound c v v0 res res'); auto.
-  apply (combine_comparison_ccompu_sound c v v0 res res'); auto.
+  apply (combine_comparison_cmp_sound valu c v v0 res res'); auto.
+  apply (combine_comparison_cmpu_sound valu m c v v0 res res'); auto.
 Qed.
 
 Theorem combine_addr_sound:
