x86/CombineOpproof.v
@@ -119,31 +119,6 @@ Proof.
   simpl; eapply combine_compimm_eq_1_sound; eauto.
 Qed.
 
-
-Lemma combine_comparison_ccomp_sound:
-  forall c x y res res',
-  combine_comparison c x y = Some res' ->
-  eval_condition (Ccomp c) (valu x :: valu y :: nil) m = Some res ->
-  res = res'.
-Proof.
-  unfold combine_comparison. intros.
-  destruct c, (eq_valnum x y); inv H; destruct (valu y); inv H0;
-  try rewrite Int.eq_true; auto;
-  unfold Int.lt; rewrite zlt_false; auto; lia.
-Qed.
-
-Lemma combine_comparison_ccompl_sound:
-  forall c x y res res',
-  combine_comparison c x y = Some res' ->
-  eval_condition (Ccompl c) (valu x :: valu y :: nil) m = Some res ->
-  res = res'.
-Proof.
-  unfold combine_comparison. intros.
-  destruct c, (eq_valnum x y); inv H; destruct (valu y); inv H0;
-  try rewrite Int64.eq_true; auto;
-  unfold Int64.lt; rewrite zlt_false; auto; lia.
-Qed.
-
 Theorem combine_cond'_sound:
   forall cond args res res',
   combine_cond' cond args = Some res' ->
@@ -152,8 +127,10 @@ Theorem combine_cond'_sound:
 Proof.
   intros.  unfold combine_cond' in *.
   destruct cond; inv H; destruct args; inv H2; destruct args; inv H1; destruct args; inv H2.
-  apply (combine_comparison_ccomp_sound c v v0 res res'); auto.
-  apply (combine_comparison_ccompl_sound c v v0 res res'); auto.
+  apply (combine_comparison_cmp_sound valu c v v0 res res'); auto.
+  apply (combine_comparison_cmpu_sound valu m c v v0 res res'); auto.
+  apply (combine_comparison_cmpl_sound valu c v v0 res res'); auto.
+  apply (combine_comparison_cmplu_sound valu m c v v0 res res'); auto.
 Qed.
 
 Theorem combine_addr_32_sound:
